src/protocol/DNS.Protocol.Parser.EverParseAdapter.fst
@@ -24,6 +24,8 @@ let generated_dns_uncompressed_question_a_answer_packet_validator_linked : bool 
 
 let generated_dns_uncompressed_question_aaaa_answer_packet_validator_linked : bool = true
 
+let generated_dns_uncompressed_question_two_a_answer_packet_validator_linked : bool = true
+
 let generated_dns_uncompressed_question_name_rdata_answer_packet_validator_linked : bool = true
 
 let generated_dns_uncompressed_question_compressed_name_rdata_answer_packet_validator_linked : bool = true
@@ -74,6 +76,13 @@ let generated_dns_uncompressed_question_a_answer_packet_validator qname_length r
 
 let generated_dns_uncompressed_question_aaaa_answer_packet_validator qname_length rr_name_length =
   DNSProtocol.validate__dns_uncompressed_question_aaaa_answer_packet qname_length rr_name_length
+
+let generated_dns_uncompressed_question_two_a_answer_packet_validator
+    qname_length first_rr_name_length second_rr_name_length =
+  DNSProtocol.validate__dns_uncompressed_question_two_a_answer_packet
+    qname_length
+    first_rr_name_length
+    second_rr_name_length
 
 let generated_dns_uncompressed_question_name_rdata_answer_packet_validator
     qname_length rr_name_length rdata_name_length expected_rtype =
